src/re.lean
@@ -5,10 +5,11 @@ namespace pca
 
 universe variable u
 variables {α : Type u}
+variables [pca α]
 
 namespace set
 
-inductive prec [pca α] (A : set α) : set α
+inductive prec (A : set α) : set α
 | rel {a} : a ∈ A → prec a
 | k : prec k
 | s : prec s
@@ -16,11 +17,11 @@ inductive prec [pca α] (A : set α) : set α
 notation `ℰ` := prec
 notation `ℰ₀` := prec ∅
 
-def recursive (A : set α) [pca α] : set α := {x | x ∈ prec A ∧ tot x}
+def recursive (A : set α) : set α := {x | x ∈ prec A ∧ tot x}
 notation `ℛ` := recursive
 notation `ℛ₀` := recursive ∅
 
-lemma pr_subset [pca α] {A B : set α} {x : α} (hx : x ∈ ℰ A) (h : A ⊆ B) : x ∈ ℰ B :=
+lemma pr_subset {A B : set α} {x : α} (hx : x ∈ ℰ A) (h : A ⊆ B) : x ∈ ℰ B :=
 begin
   induction hx with a ha a b c e ha hb iha ihb,
   { exact prec.rel (h ha),},
@@ -29,20 +30,20 @@ begin
   { exact prec.mul e iha ihb, },
 end
 
-lemma pr0_subset [pca α] {A : set α} {a : α} (ha : a ∈ (ℰ₀ : set α)) : a ∈ ℰ A :=
+lemma pr0_subset {A : set α} {a : α} (ha : a ∈ (ℰ₀ : set α)) : a ∈ ℰ A :=
 pr_subset ha (by { simp, })
 
-lemma recuraive.k [pca α] (A : set α) : k ∈ ℛ A := ⟨prec.k, ktot⟩
-lemma recuraive.s [pca α] (A : set α) : s ∈ ℛ A := ⟨prec.s, stot⟩
+lemma recuraive.k (A : set α) : k ∈ ℛ A := ⟨prec.k, ktot⟩
+lemma recuraive.s (A : set α) : s ∈ ℛ A := ⟨prec.s, stot⟩
 
-lemma prec.const (A : set α) [pca α] {a : α} : a ∈ (ℰ A : set α) → 𝐤 a ∈ (ℰ A : set α) :=
+lemma prec.const (A : set α) {a : α} : a ∈ (ℰ A : set α) → 𝐤 a ∈ (ℰ A : set α) :=
 begin
   assume h : a ∈ ℰ A,
   have l0 : ↓k * ↓a = ↓𝐤 a, { simp, },
   show 𝐤 a ∈ ℰ A, from prec.mul l0 prec.k h,
 end
 
-lemma prec.subst [pca α] (A : set α) {a b : α} :
+lemma prec.subst (A : set α) {a b : α} :
   a ∈ ℰ A → b ∈ ℰ A → 𝐬 a b ∈ ℰ A :=
 begin
   assume (ha : a ∈ ℰ A) (hb : b ∈ ℰ A),
@@ -52,10 +53,10 @@ begin
   show 𝐬 a b ∈ ℰ A, from prec.mul l2 l1 hb,
 end
 
-lemma prec.i [pca α] {A : set α} : i ∈ ℰ A := prec.subst A prec.k prec.k
-lemma recursive.i [pca α] (A : set α) : i ∈ (ℛ A : set α) := ⟨prec.i, itot⟩
+lemma prec.i {A : set α} : i ∈ ℰ A := prec.subst A prec.k prec.k
+lemma recursive.i (A : set α) : i ∈ (ℛ A : set α) := ⟨prec.i, itot⟩
 
-inductive lambdar [pca α] (A : set α) 
+inductive lambdar (A : set α) 
 | var : ℕ → lambdar
 | com {a : α} : a ∈ ℰ A → lambdar
 | app : lambdar → lambdar → lambdar
@@ -64,20 +65,20 @@ prefix `&₀`:max := lambdar.com
 notation `k₀` := &₀prec.k
 notation `s₀` := &₀prec.s
 notation `i₀` := &₀prec.i
-instance lambdar_mul {A : set α} [pca α] : has_mul (lambdar A) := ⟨lambdar.app⟩
+instance lambdar_mul {A : set α} : has_mul (lambdar A) := ⟨lambdar.app⟩
 
-def lamr [pca α] {A : set α} (n : ℕ) : lambdar A → lambdar A
+def lamr {A : set α} (n : ℕ) : lambdar A → lambdar A
 | #₀m     := if n = m then i₀ else k₀ * #₀m
 | &₀h     := k₀ * lambdar.com h
 | (l * m) := s₀ * (lamr l) * (lamr m)
 notation `Λ₀`x`,` := lamr x 
 
-def exprr [pca α] (A : set α): lambdar A → option α
+def exprr (A : set α): lambdar A → option α
 | #₀x := ↓k
 | (@lambdar.com _ _ _ e _) := ↓e
 | (l * m) := (exprr l) * (exprr m)
 
-lemma lambdar_defined [pca α] {A : set α} (n : ℕ) : ∀ (e : lambdar A), defined (exprr A (Λ₀ n, e))
+lemma lambdar_defined {A : set α} (n : ℕ) : ∀ (e : lambdar A), defined (exprr A (Λ₀ n, e))
 | #₀e := begin
     cases (eq.decidable n e),
     { simp[lamr, exprr, if_neg h], exact rfl, },
@@ -96,7 +97,7 @@ lemma lambdar_defined [pca α] {A : set α} (n : ℕ) : ∀ (e : lambdar A), def
 
 notation n` -[`A`]→ ` l := option.get (@lambdar_defined _ _ A n l)
 
-lemma lambdar_pr [pca α] {A : set α} :
+lemma lambdar_pr {A : set α} :
   ∀ {e : lambdar A} (h : defined (exprr A e) = tt), option.get h ∈ (ℰ A : set α)
 | #₀_ _ := prec.k
 | &₀p _ := p
@@ -109,39 +110,63 @@ lemma lambdar_pr [pca α] {A : set α} :
     show option.get h ∈ ℰ A, from prec.mul e lpr mpr,
   end
 
-lemma lambda_pr0 [pca α] {A : set α} (n : ℕ) (e : lambdar A) : (n -[A]→ e) ∈ (ℰ A : set α) := lambdar_pr _
+@[simp] lemma lambda_pr0 {A : set α} (n : ℕ) (e : lambdar A) : (n -[A]→ e) ∈ (ℰ A : set α) := lambdar_pr _
 
 namespace recursion_pr
 
-def d [pca α] : α := 0 -[∅]→ (Λ₀ 1, (#₀0 * #₀0 * #₀1))
-def dpr [pca α] : d ∈ (ℰ₀ : set α) := lambda_pr0 _ _
+def d : α := 0 -[∅]→ (Λ₀ 1, (#₀0 * #₀0 * #₀1))
+def dpr : d ∈ (ℰ₀ : set α) := lambda_pr0 _ _
 
-def v [pca α]: α := 0 -[∅]→ (Λ₀ 1, (#₀0 * (&₀dpr * #₀1)))
-def vpr [pca α] : v ∈ (ℰ₀ : set α) := lambda_pr0 _ _
+def v: α := 0 -[∅]→ (Λ₀ 1, (#₀0 * (&₀dpr * #₀1)))
+def vpr : v ∈ (ℰ₀ : set α) := lambda_pr0 _ _
 
-def n [pca α] : α := 0 -[∅]→ (&₀dpr * (&₀vpr * #₀0))
-def npr [pca α] : n ∈ (ℰ₀ : set α) := lambda_pr0 _ _
+def n : α := 0 -[∅]→ (&₀dpr * (&₀vpr * #₀0))
+def npr : n ∈ (ℰ₀ : set α) := lambda_pr0 _ _
 
-lemma fixpoint_eq_n [pca α] : @fixpoint α _ = n :=
+lemma fixpoint_eq_n : @fixpoint α _ = n :=
 by { simp [fixpoint,recursion.n,n,recursion.d,recursion.v,d,v], refl, }
 
-lemma fixpoint_pr [pca α] : fixpoint ∈ (ℰ₀ : set α) := by { rw fixpoint_eq_n, exact npr, }
-lemma fixpoint_re [pca α] : fixpoint ∈ (ℛ₀ : set α) := ⟨fixpoint_pr, recursion.ntot⟩
+lemma fixpoint_pr : fixpoint ∈ (ℰ₀ : set α) := by { rw fixpoint_eq_n, exact npr, }
+lemma fixpoint_re : fixpoint ∈ (ℛ₀ : set α) := ⟨fixpoint_pr, recursion.ntot⟩
 
 end recursion_pr
 
-class numbering (α : Type u) [pca α]
-(code : α → ℕ)
-(decode : ℕ → α)
-(nat_pr : ∀ n : ℕ, decode n ∈ (ℰ₀ : set α))
-(decode_code : ∀ x : α, x ∈ (ℰ₀ : set α) → decode (code x) = x)
-(code_decode : ∀ n : ℕ, code (decode n) = n)
+def reducible (A : set α) (f g : α) : Prop := ∃ e : α, e ∈ ℰ A ∧ ↓e * ↓g = ↓f 
+def T_reducible (f g : α) : Prop := reducible ∅ f g
+infix ` ≤_T `:80 := T_reducible
+infix ` ≡_T `:80 := λ f g, f ≤_T g ∧ g ≤_T f
 
-def Kl [pca α] : set α := {x : α | defined (↓x * ↓x)}
-def K (A : set α) [pca α] := {x : α | x ∈ A ∧ defined (↓x * ↓x)}
-def representable [pca α] (A : set α) : set (set α) := {B | ∃ e, e ∈ A ∧ B = {x | defined (↓e * ↓x)}}
+@[refl] lemma T_reducible.refl (a : α) : a ≤_T a :=
+by { use i, split, exact prec.i, simp, }
+
+@[trans] lemma T_reducible.trans (a b c : α) (hab : a ≤_T b) (hbc : b ≤_T c) : a ≤_T c :=
+begin
+  rcases hab with ⟨e_ab, ⟨e_ab_pr, heab⟩⟩,
+  rcases hbc with ⟨e_bc, ⟨e_bc_pr, hebc⟩⟩,
+  let e_ac := (0 -[∅]→ &₀e_ab_pr * (&₀e_bc_pr * #₀0)),
+  use e_ac,
+  split,
+  { show e_ac ∈ ℰ₀, simp, },
+  { show ↓e_ac * ↓c = ↓a, simp [lamr, exprr, heab, hebc], },
+end
+
+namespace jump
+
+def jump_pred (A : set α) (j : α) : Prop := 
+(∀ x, x ∈ ℰ A → ↓j * ↓x = ↓(if defined (↓x * ↓x) then combinator.top else combinator.bot))
+theorem jhjhj (A : set α) (j : α) (hj : jump_pred A j) : j ∉ ℰ A :=
+begin
+  assume h : j ∈ ℰ A,
+  let 
+end 
+
+end jump
+
+def Kl : set α := {x : α | defined (↓x * ↓x)}
+def K (A : set α) := {x : α | x ∈ A ∧ defined (↓x * ↓x)}
+def representable (A : set α) : set (set α) := {B | ∃ e, e ∈ A ∧ B = {x | defined (↓e * ↓x)}}
 notation A` is_representable_in `B := A ∈ representable B
-def re_set [pca α] (A : set α) : Prop := ∃ e : α, e ∈ (ℰ₀ : set α) ∧ A = {x | defined (↓e * ↓x)}
+def re_set (A : set α) : Prop := ∃ e : α, e ∈ (ℰ₀ : set α) ∧ A = {x | defined (↓e * ↓x)}
 
 lemma neg_p_iff_negp (P : Prop) : ¬(P ↔ ¬P) := 
 begin
@@ -150,7 +175,7 @@ begin
   exact h₂ (h₁ h₂),
 end
 
-lemma K_re [pca α] : Kl is_representable_in (ℰ₀ : set α) :=
+lemma K_re : Kl is_representable_in (ℰ₀ : set α) :=
 begin
   use (0 ↦ #0 * #0),
   have h : ∀ x : α, expr (Λ 0, (#0 * #0)) * ↓x = ↓x * ↓x, { intros x, simp [lam, expr], },
@@ -164,7 +189,7 @@ begin
   { unfold Kl, simp, assume xh, rw ← h x, exact xh, },
 end
 
-lemma compl_K_nre [pca α] : ¬ re_set (Klᶜ : set α) :=
+lemma compl_K_nre : ¬ re_set (Klᶜ : set α) :=
 begin
   rintro ⟨e, h⟩,
   apply neg_p_iff_negp (e ∈ (Kl : set α)),
